finally making progress on total_order refactoring

lib/Base/total_order.i.dfy
@@ -751,6 +751,25 @@ abstract module Total_Order {
   }
 }*/
 
+
+abstract module Total_Order_Implementation {
+  import opened Ord : Total_Order
+  import opened NativeTypes
+    
+  method cmp(a: Element, b: Element) returns (c: int32)
+    ensures c < 0 ==> lt(a, b)
+    ensures c > 0 ==> lt(b, a)
+    ensures c == 0 ==> a == b
+    
+  method IsSorted(s: seq<Ord.Element>) returns (result: bool)
+    ensures result == Ord.IsSorted(s)
+  {
+    assume false;
+    result := false;
+  }
+}
+
+
 module Integer_Order refines Total_Order {
   type Element = int
 
@@ -779,11 +798,6 @@ module Uint32_Order refines Total_Order {
   predicate method {:opaque} ltedef(a: Element, b: Element) {
     a <= b
   }
-
-  method cmp(a: Element, b: Element) returns (c: int32)
-  {
-    return if a < b then -1 else if a > b then 1 else 0;
-  }
 }
 
 module Uint64_Order refines Total_Order {
@@ -799,11 +813,6 @@ module Uint64_Order refines Total_Order {
   predicate method {:opaque} ltedef(a: Element, b: Element) {
     a <= b
   }
-
-  method cmp(a: Element, b: Element) returns (c: int32)
-  {
-    return if a < b then -1 else if a > b then 1 else 0;
-  }
 }
 
 
@@ -818,11 +827,6 @@ module Char_Order refines Total_Order {
 
   predicate method ltedef(a: Element, b: Element) {
     a <= b
-  }
-
-  method cmp(a: Element, b: Element) returns (c: int32)
-  {
-    return if a < b then -1 else if a > b then 1 else 0;
   }
 }
 
@@ -853,13 +857,6 @@ module Byte_Order refines Total_Order {
 
   predicate method {:opaque} ltedef(a: Element, b: Element) {
     a <= b
-  }
-
-  method cmp(a: Element, b: Element) returns (c: int32)
-  {
-    reveal_lte();
-    reveal_ltedef();
-    return if a < b then -1 else if a > b then 1 else 0;
   }
 }
 
@@ -924,198 +921,10 @@ module Lexicographic_Byte_Order refines Total_Order {
     }
   }
 
-  method cmp(a: Element, b: Element) returns (c: int32)
-    ensures c < 0 ==> lt(a, b)
-    ensures c > 0 ==> lt(b, a)
-    ensures c == 0 ==> a == b
-  {
-    c := NativeArrays.ByteSeqCmpByteSeq(a, b);
-  }
-
   lemma EmptyLte(x: Element)
   ensures lte([], x)
   {
     SeqComparison.reveal_lte();
-  }
-
-  // TODO Ideally we would put these methods in the abstract class
-  // (since they could apply to any kind of Element)
-  // But then our c++ backend would not be able to compile
-  // Integer_Total_Order which uses the `int` type.
-
-  method ArrayLargestLtePlus1Linear(run: array<Element>, start: uint64, end: uint64, needle: Element) returns (posplus1: uint64)
-    requires 0 <= start as int <= end as int <= run.Length < Uint64UpperBound() / 2
-    requires IsSorted(run[start..end]);
-    ensures posplus1 as int == start as int + LargestLte(run[start..end], needle) + 1
-  {
-    var i: uint64 := start;
-    var t;
-    if i < end {
-      t := cmp(run[i], needle);
-    }
-    while i < end && t <= 0
-      invariant start <= i <= end
-      invariant forall j :: start <= j < i ==> lte(run[j], needle)
-      invariant i < end ==> (t <= 0 <==> lte(run[i], needle))
-    {
-      i := i + 1;
-      if i < end {
-        t := cmp(run[i], needle);
-      }
-    }
-    forall j | i <= j < end
-      ensures lt(needle, run[j])
-    {
-      reveal_IsSorted();
-      assert lt(needle, run[i]);
-      assert lte(run[i], run[j]);
-    }
-    LargestLteIsUnique(run[start..end], needle, i as int - start as int - 1);
-    posplus1 := i;
-  }
-
-  method ArrayLargestLtePlus1(run: array<Element>, start: uint64, end: uint64, needle: Element) returns (posplus1: uint64)
-    requires 0 <= start as int <= end as int <= run.Length < Uint64UpperBound() / 2
-    requires IsSorted(run[start..end]);
-    ensures posplus1 as int == start as int + LargestLte(run[start..end], needle) + 1
-  {
-    reveal_IsSorted();
-    var lo := start;
-    var hi := end + 1;
-    while 1 < hi - lo 
-      invariant start <= lo < hi <= end + 1
-      invariant forall i :: start <= i < lo ==> lte(run[i], needle)
-      invariant forall i :: hi - 1 <= i < end ==> lt(needle, run[i])
-      decreases hi - lo
-    {
-      var mid := (lo + hi) / 2;
-      var t := cmp(run[mid-1], needle);
-      if t <= 0 {
-        lo := mid;
-      } else {
-        hi := mid;
-      }
-    }
-    var i: uint64 := lo;
-    /*
-    var t;
-    if i < hi {
-      t := cmp(run[i], needle);
-    }
-    while i < hi && t <= 0
-      invariant start <= i <= end
-      invariant forall j :: start <= j < i ==> lte(run[j], needle)
-      invariant i < hi ==> (t <= 0 <==> lte(run[i], needle))
-    {
-      i := i + 1;
-      if i < hi {
-        t := cmp(run[i], needle);
-      }
-    }
-    forall j | i <= j < end
-      ensures lt(needle, run[j])
-    {
-      reveal_IsSorted();
-      assert lt(needle, run[i]);
-      assert lte(run[i], run[j]);
-    }
-    */
-    LargestLteIsUnique(run[start..end], needle, i as int - start as int - 1);
-    posplus1 := i;
-  }
-  
-  method ArrayLargestLtPlus1(run: array<Element>, start: uint64, end: uint64, needle: Element) returns (posplus1: uint64)
-    requires 0 <= start as int <= end as int <= run.Length < Uint64UpperBound() / 2
-    requires IsSorted(run[start..end]);
-    ensures posplus1 as int == start as int + LargestLt(run[start..end], needle) + 1
-  {
-    reveal_IsSorted();
-    var lo := start;
-    var hi := end + 1;
-    while 1 < hi - lo 
-      invariant start <= lo < hi <= end + 1
-      invariant forall i :: start <= i < lo ==> lt(run[i], needle)
-      invariant forall i :: hi - 1 <= i < end ==> lte(needle, run[i])
-      decreases hi - lo
-    {
-      var mid := (lo + hi) / 2;
-      var t := cmp(run[mid-1], needle);
-      if t < 0 {
-        lo := mid;
-      } else {
-        hi := mid;
-      }
-    }
-    var i: uint64 := lo;
-    /*
-    var t;
-    if i < hi {
-      t := cmp(run[i], needle);
-    }
-    while i < hi && t < 0
-      invariant start <= i <= end
-      invariant forall j :: start <= j < i ==> lt(run[j], needle)
-      invariant i < hi ==> (t < 0 <==> lt(run[i], needle))
-    {
-      i := i + 1;
-      if i < hi {
-        t := cmp(run[i], needle);
-      }
-    }
-    */
-    LargestLtIsUnique(run[start..end], needle, i as int - start as int - 1);
-    posplus1 := i;
-  }
-
-  method ComputeLargestLte(run: seq<Element>, needle: Element) returns (res : int64)
-    requires |run| < 0x4000_0000_0000_0000
-    requires IsSorted(run)
-    ensures res as int == LargestLte(run, needle)
-  {
-    var lo: int64 := 0;
-    var hi: int64 := |run| as int64;
-    while lo < hi
-    invariant 0 <= lo as int <= hi as int <= |run|
-    invariant 1 <= lo as int ==> lte(run[lo-1], needle)
-    invariant hi as int < |run| ==> lt(needle, run[hi])
-    invariant lo <= hi
-    decreases hi - lo
-    {
-      var mid := (lo + hi) / 2;
-      var c := cmp(run[mid], needle);
-      if (c > 0) {
-        hi := mid;
-      } else {
-        lo := mid+1;
-      }
-    }
-
-    return lo - 1;
-  }
-    
-  method ComputeLargestLt(run: seq<Element>, needle: Element) returns (res : int64)
-    requires |run| < 0x4000_0000_0000_0000
-    requires IsSorted(run)
-    ensures res as int == LargestLt(run, needle)
-  {
-    var lo: int64 := 0;
-    var hi: int64 := |run| as int64;
-    while lo < hi
-    invariant 0 <= lo as int <= hi as int <= |run|
-    invariant 1 <= lo as int ==> lt(run[lo-1], needle)
-    invariant hi as int < |run| ==> lte(needle, run[hi])
-    decreases hi - lo
-    {
-      var mid := (lo + hi) / 2;
-      var c := cmp(run[mid], needle);
-      if (c < 0) {
-        lo := mid+1;
-      } else {
-        hi := mid;
-      }
-    }
-
-    return lo - 1;
   }
 
 }
