lib/Buckets/PackedStringArrayMarshalling.i.dfy
@@ -1,32 +1,73 @@
+include "../Base/Option.s.dfy"
 include "../Marshalling/GenericMarshalling.i.dfy"
-include "PackedStringArray"
+include "PackedStringArray.i.dfy"
 
 module PackedStringArrayMarshalling {
+  import opened Options
   import opened PackedStringArray
   import opened GenericMarshalling
 
   function method grammar() : G
-  ensures ValidGrammar(PSAGrammar())
+  ensures ValidGrammar(grammar())
   {
     GTuple([
       GUint32Array, // offsets
-      GbyteArray    // string bytes
+      GByteArray    // string bytes
     ])
   }
 
-  method toVal(psa: PSA.Psa)
-    returns (v: V)
-    requires PSA.WF(psa)
-    ensures ValidInGrammar(grammar(), v)
+  function  fromVal(v: V) : (opsa: Option<Psa>)
+    requires ValInGrammar(v, grammar())
+    ensures opsa.Some? ==> WF(opsa.value)
   {
-    v := VTuple([VUint32Array(psa.offsets), VByteArray(psa.data)]);
+    assert ValInGrammar(v.t[0], GUint32Array);
+    assert ValInGrammar(v.t[1], GByteArray);
+    var offsets := v.t[0].va;
+    var data := v.t[1].b;
+    var psa := Psa(offsets, data);
+    if WF(psa) then
+      Some(psa)
+    else
+      None
+  }
+  
+  function toVal(psa: Psa) : (v: V)
+    requires WF(psa)
+    ensures ValInGrammar(v, grammar())
+    ensures fromVal(v) == Some(psa)
+  {
+    VTuple([VUint32Array(psa.offsets), VByteArray(psa.data)])
   }
 
-  method fromVal(v: V)
-    returns (psa: PSA.Psa)
-    requires ValidInGrammar(grammar(), v)
-    ensures PSA.WF(psa)
+  method computeWF(psa: Psa) return (result: bool)
+    ensures result == WF(psa)
   {
-    v := VTuple([VUint32Array(psa.offsets), VByteArray(psa.data)]);
+    
   }
+  
+  method fromVal(v: V)
+    returns (psa: Option<Psa>)
+    requires ValInGrammar(v, grammar())
+    ensures psa.Some? ==> WF(psa.value)
+  {
+    assert ValInGrammar(v.t[0], GUint32Array);
+    assert ValInGrammar(v.t[1], GByteArray);
+    var offsets := v.t[0].va;
+    var data := v.t[1].b;
+    var psa := Psa(offsets, data);
+    if WF(psa) then
+      Some(psa)
+    else
+      None
+  }
+
+  // method ToVal(psa: Psa)
+  //   returns (v: V)
+  //   requires WF(psa)
+  //   ensures ValInGrammar(v, grammar())
+  //   ensures v == Val(psa)
+  // {
+  //   v := VTuple([VUint32Array(psa.offsets), VByteArray(psa.data)]);
+  // }
+
 }
